Type.thy
@@ -1,0 +1,11 @@
+theory Type
+imports Main
+begin
+
+datatype type = 
+  Base
+| Arrow type type
+| Record "type list"
+| Variant "type list"
+
+end
